src/lib/kernel/Kuiper.Kernel.OnlineSoftmaxDotprod.fsti
@@ -1,0 +1,34 @@
+module Kuiper.Kernel.OnlineSoftmaxDotprod
+
+#lang-pulse
+open Kuiper
+open Kuiper.Seq.Common
+open Kuiper.Array1
+open Kuiper.Tensor.Layout { ctlayout }
+module KS = Kuiper.Spec.Softmax
+open Kuiper.DotProd
+
+inline_for_extraction noextract
+fn softmax_dotprod
+  (#et : Type0) {| floating et, real_like et, floating_real_like et |}
+  (len : szp{len <= max_blocks * max_threads})
+  (#l : Kuiper.Array1.layout len) {| ctlayout l |}
+  (a : array1 et l)
+  (b : array1 et l)
+  (r : gpu_ref et)
+  (#va : erased (lseq et len))
+  (#vb : erased (lseq et len))
+  (ra : erased (lseq real len) { va %~ ra })
+  (rb : erased (lseq real len) { vb %~ rb })
+  (#fa #fb : perm)
+  (#_: squash (seq_forallb not_nan va))
+  (tid : szlt len)
+  ()
+  preserves
+    gpu **
+    a |-> Frac fa va **
+    b |-> Frac fb vb
+  returns
+    res : et
+  ensures
+    pure (res %~ seq_dotprod (KS.softmax_real ra) rb)
